Tweaks to forward_while, forward_call.
forward_while tweaked slightly to clean up the "HRE" assumption:
after the loop, the "loop condition false" is now cleaned up by
do_repr_inj.  This improves the proof slightly, which may
cause incompatibility (no change in progs,hmac; one change in sha).

forward call, in the case where the funspec's postcondition 			did NOT start with an existential (EX), previously created
an (EX vret: val, ...).  Now it intros that existential and
eliminates vret by doing a subst.  Some proofs need to be adjusted
by deleting "Intros vret; subst vret" after the forward_call.

progs,sha,hmac,tweetnacl all brought up to date.

floyd/call_lemmas.v
@@ -1409,12 +1409,17 @@ apply andp_left2. apply andp_left1.
  rewrite fold_right_sepcon_app. auto.
 Qed.  
 
+Definition eq_no_post (x v: val) : Prop := x=v.
+(* The purpose of eq_no_post is to "mark" the proposition
+  in forward_call_idxxx lemmas so that the after-the-call
+  can treat this one specially *)
+
 Lemma no_post_exists:
  forall v P Q R,
    PROPx P (LOCALx (temp ret_temp v :: Q) (SEPx R)) =
-   EX x:val, PROPx ((x=v) :: P) (LOCALx (temp ret_temp x :: Q) (SEPx R)).
+   EX x:val, PROPx (eq_no_post x v :: P) (LOCALx (temp ret_temp x :: Q) (SEPx R)).
 Proof.
-intros.
+intros. unfold eq_no_post.
 apply pred_ext.
 apply exp_right with v.
 apply andp_derives; auto.
